low/Rinit.v
@@ -135,7 +135,7 @@ Definition InitNames_shorcuts S :=
   let%success R_RestartToken := mkSymMarker globals S str using S in
   (** Some ignored global values: [R_InBCInterpreter], [R_CurrentExpression] **)
   let (S, NA_STRING) := alloc_vector_char globals S (string_to_list "NA") in
-  map%gp NA_STRING with @NBits.write_nbit 16 5 ltac:(NBits.nbits_ok) true using S in
+  map%gp NA_STRING with @write_nbit 16 5 ltac:(nbits_ok) true using S in
   let (S, R_BlankString) := mkChar globals S "" in
   let%success R_BlankScalarString := ScalarString globals S R_BlankString using S in
   let R_SymbolTable := R_NilValue in
@@ -243,7 +243,7 @@ Definition init_R_Toplevel S :=
       conexit := R_NilValue ;
       returnValue := NULL ;
       jumptarget := None ;
-      jumpmask := empty_context_types
+      jumpmask := empty_context_type
     |}.
 
 End Globals.
@@ -338,7 +338,7 @@ Definition empty_context := {|
     conexit := NULL ;
     returnValue := NULL ;
     jumptarget := None ;
-    jumpmask := empty_context_types
+    jumpmask := empty_context_type
   |}.
 
 (** An empty (and dummy) state **)
